Structure/Data/Notation.lean
@@ -1,0 +1,11 @@
+set_option autoBoundImplicitLocal false
+
+universes u₁ u₂ v
+
+
+
+class HasEquivalence (α : Sort u₁) (β : Sort u₂) where
+{γ : Sort v}
+(Equiv : α → β → γ)
+
+infix:25 " ≃ "  => HasEquivalence.Equiv
